\begin{algorithm}
\caption{Kahan Summation Incremental Update} 
\label{algo:kahan}
\begin{algorithmic}
\small{
\STATE //  $s_1$ and $s_2$ are partial sums, $c_1$ and $c_2$ are correction terms
\STATE \textsc{KahanIncrement}($s_1, c_1, s_2, c_2$)\{
\STATE \ \ $corrected\_s_2 = s_2 + (c_1+c_2)$
\STATE \ \ $sum=s_1+corrected\_s_2$
\STATE \ \ $correction=corrected\_s_2-(sum - s_1)$
\STATE \ \ \textbf{return} $(sum, correction)$ \}
}
\end{algorithmic}
\end{algorithm}

%\begin{algorithm}
%\caption{Kahan Summation} 
%\label{algo:kahan}
%\begin{algorithmic}
%\small{
%\STATE \textbf{KahanSum}(X: input data items)\{
%\STATE \ \ $sum=0$, $correction=0$
%\STATE \ \ \textbf{for} $i = 1 \to X.size$ 
%\STATE \ \ \ \ $(sum, correction)=\textbf{KahanAdd}(sum, correction, x_i, 0)$
%\STATE \ \ \textbf{return} $sum$ \}
%\STATE 
%\STATE //  $s_1$ and $s_2$ are partial sums, $c_1$ and $c_2$ are correction terms
%\STATE \textbf{KahanAdd}($s_1, c_1, s_2, c_2$)\{
%\STATE \ \ $corrected\_s_2 = s_2 + c_1+c_2$
%\STATE \ \ $sum=s_1+corrected\_s_2$
%\STATE \ \ $new\_c=corrected\_s_2-(sum - s_1)$
%\STATE \ \ \textbf{return} $(sum, new\_c)$ \}
%}
%\end{algorithmic}
%\end{algorithm}
